---
title: Romania TST 1999/4
description: An interesting product-to-sum trick to apply Jensen/Karamata.
date: '2024-3-2'
categories:
  - math
  - contests
published: true
---

> Let $x_1, \dots, x_n > 0$ be positive reals satisfying $x_1 \dots x_n = 1$. Prove that
> $$
> \frac{1}{n - 1 + x_1} + \frac{1}{n - 1 + x_2} + \dots + \frac{1}{n - 1 + x_n} \le 1.
> $$
> --[1999 Romania TST Question 4](https://artofproblemsolving.com/community/c6h238609p1965995)

$n = 1$ is trivial. Henceforth we assume $n \geq 2$. This looks like $\sum f(x_i)$ and ideal for Jensen/Karamata, but unfortunately we don't have $\sum x_i$ as a condition, but $\prod x_i$ instead. 

Let's force a sum condition by taking logarithms! Write $y_i = \ln(x_i)$ and $f(x) = \frac{1}{n - 1 + e^x}$. Then we wish to prove, subject to $\sum y_i = 0$,  
$$
\sum f(y_i) \leq 1
$$

Of course, we now consider the convexity of $f$. 
$$
f''(x) = (e^{2x} - (n - 1)e^x)/(e^x + n - 1)^3.
$$
$f$ has only one inflection point, namely $x = \ln(n - 1)$. We are in perfect condition to apply the $n - 1$ EV principle. We prove that there exist reals $z_1 = z_2 = \dots = z_{n - 1}$, $z_n$ also satisfying $\sum z_i = 0$ such that $\sum f(y_i) \le f(z_i)$. 

If one or less of $y_i$ lie in $(\ln(n - 1), \infty)$, we are done by Jensen's Inequality on the rest of $y_i$. Then assume for $k \geq 2$ and $y_i$ nonincreasing, exactly $y_1, y_2, \dots, y_k$ lie in $(\ln(n - 1), \infty)$, where $f$ is convex. Set $t_n = y_1 + y_2 + \dots + y_k - (k - 1)\ln(n - 1)$ and $t_1 = t_2 = \dots = t_{k - 1} = \ln(n - 1)$. Note $(t_n, t_1, t_2, \dots, t_{k - 1}) \succ (y_1, y_2, \dots, y_k)$ and by Karamata's Inequality,

$$
\sum_{i = 1}^k f(y_i) \leq f(t_n) + \sum_{i = 1}^{k - 1} f(t_i)
$$

Hence by Jensen's,
$$
\sum f(y_i) \leq f(t_n) + \sum_{i = 1}^{n - 1} f(t_i) \leq f(t_n) + (n - 1) f\left(\frac{\sum_{i = 1}^{n - 1} t_i}{n - 1}\right)
$$
So we are done setting $z_n$ accordingly.

Now without loss of generality, we may assume $y = y_1 = y_2 = \dots = y_{n - 1}$, and note $y_n = -(n - 1)y$.
It remains to prove 

$$
\frac{n - 1}{n - 1 + e^y} + \frac{1}{n - 1 + e^{-(n - 1)y}} \leq 1
$$
$$
\iff (n - 2) e^y + e^{-(n - 2)y} \geq n - 1
$$

Which is immediately obvious by Weighted Power Mean. $\blacksquare$